Tealeaves/Classes/Kleisli/DecoratedContainerMonad.v
@@ -9,7 +9,7 @@ Import List.ListNotations.
 Import ContainerFunctor.Notations.
 Import DecoratedContainerFunctor.Notations.
 
-#[local] Generalizable Variables A T W.
+#[local] Generalizable Variables A T U W.
 
 (** * Decorated container monads *)
 (******************************************************************************)
@@ -22,30 +22,28 @@ Class DecoratedContainerMonad
   `{Bindd W T T} `{Return T}
   `{ElementsCtx W T} :=
   { dconm_functor :> DecoratedMonad W T;
-    dconm_morphism_ret : forall (A : Type),
-      element_ctx_of ∘ ret (T := T) (A := A) =
-        ret (T := ctxset W);
-    dconm_morphism_bind : forall (A B : Type) (f : W * A -> T B),
-      element_ctx_of ∘ bindd f =
-        bindd (element_ctx_of ∘ f) ∘ element_ctx_of;
+    decom_hom :> DecoratedMonadHom W T (ctxset W) (@element_ctx_of W T _);
     dconm_pointwise : forall (A B : Type) (t : T A) (f g : W * A -> T B),
       (forall e a, (e, a) ∈d t -> f (e, a) = g (e, a)) -> bindd f t = bindd g t;
   }.
 
 Class DecoratedContainerMonadFull
   (W : Type) (T : Type -> Type)
-  `{Map T} `{Mapd W T} `{Bind T T}
-  `{Bindd W T T} `{Return T}
-  `{Monoid_op W} `{Monoid_unit W}
+  `{Map T}
+  `{Mapd W T}
+  `{Bind T T}
+  `{Bindd W T T}
+  `{Return T}
+  `{Monoid_op W}
+  `{Monoid_unit W}
   `{Monoid W}
   `{ElementsCtx W T} `{Elements T} :=
   { dconmf_dconm :> DecoratedContainerMonad W T;
     dconmf_functor :> DecoratedMonadFull W T;
-    dconmf_element_compat : forall (A : Type),
-      element_of (F := T) (A := A) =
-        map (F := subset) extract ∘ element_ctx_of (F := T);
+    dconmf_element_compat :> Compat_Elements_ElementsCtx;
   }.
 
+(*
 #[local] Instance tmp `{DecoratedContainerMonadFull W T} :
   DecoratedContainerFunctorFull W T.
 Proof.
@@ -74,24 +72,62 @@ Proof.
       apply dconm_pointwise.
       admit.
 Admitted.
+     *)
 
 (** * Basic properties of containers *)
 (******************************************************************************)
 Section decorated_container_monad_theory.
 
   Context
-    `{DecoratedContainerMonadFull W T}.
+    `{ret_inst : Return T}
+      `{Bindd_T_inst : Bindd W T T}
+      `{Bindd_U_inst : Bindd W T U}
+      `{Mapd_T_inst : Mapd W T}
+      `{Mapd_U_inst : Mapd W U}
+      `{Bind_T_inst : Bind T T}
+      `{Bind_U_inst : Bind T U}
+      `{Map_T_inst : Map T}
+      `{Map_U_inst : Map U}
+      `{op : Monoid_op W}
+      `{unit : Monoid_unit W}
+      `{Map_Bindd_T_inst : ! Compat_Map_Bindd W T T}
+      `{Bind_Bindd_T_inst : ! Compat_Bind_Bindd W T T}
+      `{Mapd_Bindd_T_inst : ! Compat_Mapd_Bindd W T T}
+      `{Map_Bindd_inst : ! Compat_Map_Bindd W T U}
+      `{Bind_Bindd_inst : ! Compat_Bind_Bindd W T U}
+      `{Mapd_Bindd_inst : ! Compat_Mapd_Bindd W T U}
+      `{Module_inst : ! DecoratedRightModule W T U}
+      `{ElementsCtx_T_inst : ElementsCtx W T}
+      `{ElementsCtx_U_inst : ElementsCtx W U}
+      `{Elements_T_inst : Elements T}
+      `{Elements_U_inst : Elements U}
+      `{Monad_inst : ! DecoratedContainerMonad W T}
+      `{! Compat_Elements_ElementsCtx (E := W) (T := T)}.
 
   Variables (A B : Type).
 
   Implicit Types (t : T A) (b : B) (w : W) (a : A).
+
+  Lemma dconm_morphism_ret : forall (A : Type),
+      element_ctx_of ∘ ret (T := T) (A := A) =
+        ret (T := ctxset W).
+  Proof.
+    apply kmond_hom_ret.
+  Qed.
+
+  Lemma dconm_morphism_bind : forall (A B : Type) (f : W * A -> T B),
+      element_ctx_of ∘ bindd f =
+        bindd (U := ctxset W) (element_ctx_of ∘ f) ∘ element_ctx_of (F := T).
+  Proof.
+    apply kmond_hom_bind.
+  Qed.
 
   Theorem ind_ret_iff : forall {A : Type} (w : W) (a1 a2 : A),
       (w, a1) ∈d ret (T := T) a2 <-> w = Ƶ /\ a1 = a2.
   Proof.
     intros.
     compose near a2 on left.
-    rewrite dconm_morphism_ret.
+    rewrite kmond_hom_ret.
     unfold_ops @Return_ctxset.
     intuition.
   Qed.
@@ -102,8 +138,9 @@ Section decorated_container_monad_theory.
                    exists wb : W, (wb, b) ∈d f (wa, a) /\
                                w = wa ● wb.
   Proof.
-    introv. compose near t on left.
-    rewrite dconm_morphism_bind.
+    introv.
+    compose near t on left.
+    rewrite kmond_hom_bind.
     reflexivity.
   Qed.
 
@@ -114,18 +151,18 @@ Section decorated_container_monad_theory.
                                w = wa ● wb.
   Proof.
     introv.
-    rewrite kmondf_bind_compat.
+    rewrite bind_to_bindd.
     rewrite ind_bindd_iff.
     reflexivity.
   Qed.
 
   Corollary in_bindd_iff : forall t f b,
-      b ∈ bindd f t <->
+      b ∈ bindd (U := T) f t <->
         exists (wa : W) (a : A),
           (wa, a) ∈d t /\ b ∈ f (wa, a).
   Proof.
     introv.
-    setoid_rewrite (element_ctx_iff_element W T).
+    setoid_rewrite element_ctx_iff_element.
     setoid_rewrite ind_bindd_iff.
     split.
     - intros [w [wa [a [Hin [wb [Hin' Heq]]]]]].
